Added monomorphisation proof and rejigged the embedding
This commit includes the monomorphisation proof for the general for loop
"repeat". The embeddings in the update and value semantics were modified
so that this could be proved, and the other proofs were updated
to account for these changes.

cogent/examples/repeat/RepeatUpdate.thy
@@ -37,26 +37,17 @@ definition \<xi>0 :: "(funtyp, abstyp, ptrtyp) uabsfuns"
 "\<xi>0 f x y = False"
 end
 
-\<comment>\<open>Need to add @{term "\<forall>v. (\<xi>' , [v] \<turnstile> (\<sigma>, App f (Var 0)) \<Down>! (\<sigma>, UPrim (LBool True))) \<longrightarrow> \<not>(\<xi>' , [v] \<turnstile> (\<sigma>, App f (Var 0)) \<Down>! (\<sigma>, UPrim (LBool False))) " }\<close>
-thm contrapos_imp
-
-fun repeat_bod
+fun urepeat_bod
   where
-"repeat_bod _ 0 _ _ \<sigma> \<sigma>' _ acc _ _ ret = (\<sigma> = \<sigma>' \<and> acc = ret)" |
-"repeat_bod \<xi>' (Suc n) f g \<sigma> \<sigma>' \<tau>a acc \<tau>o obsv ret =
-  (if (\<xi>' , [URecord [(acc, type_repr (bang \<tau>a)), (obsv, type_repr \<tau>o)]] 
-      \<turnstile> (\<sigma>, App f (Var 0)) \<Down>! (\<sigma>, UPrim (LBool True))) \<and>
-      \<not>(\<xi>' , [URecord [(acc, type_repr (bang \<tau>a)), (obsv, type_repr \<tau>o)]] 
-      \<turnstile> (\<sigma>, App f (Var 0)) \<Down>! (\<sigma>, UPrim (LBool False)))
-    then \<sigma> = \<sigma>' \<and> acc = ret
-  else if (\<xi>' , [URecord [(acc, type_repr (bang \<tau>a)), (obsv, type_repr \<tau>o)]] 
-      \<turnstile> (\<sigma>, App f (Var 0)) \<Down>! (\<sigma>, UPrim (LBool False))) \<and>
-      \<not>(\<xi>' , [URecord [(acc, type_repr (bang \<tau>a)), (obsv, type_repr \<tau>o)]] 
-      \<turnstile> (\<sigma>, App f (Var 0)) \<Down>! (\<sigma>, UPrim (LBool True)))
-    then (\<exists>\<sigma>'' acc'. (\<xi>' , [URecord [(acc, type_repr \<tau>a), (obsv, type_repr \<tau>o)]] 
+"urepeat_bod _ 0 _ _ \<sigma> \<sigma>' _ acc _ _ ret = (\<sigma> = \<sigma>' \<and> acc = ret)" |
+"urepeat_bod \<xi>' (Suc n) f g \<sigma> \<sigma>' \<tau>a acc \<tau>o obsv ret =
+  (\<exists>b. (\<xi>' , [URecord [(acc, type_repr (bang \<tau>a)), (obsv, type_repr \<tau>o)]] 
+      \<turnstile> (\<sigma>, App f (Var 0)) \<Down>! (\<sigma>, UPrim (LBool b))) \<and>
+    (if b then \<sigma> = \<sigma>' \<and> acc = ret
+     else (\<exists>\<sigma>'' acc'. (\<xi>' , [URecord [(acc, type_repr \<tau>a), (obsv, type_repr \<tau>o)]] 
         \<turnstile> (\<sigma>, App g (Var 0)) \<Down>! (\<sigma>'', acc')) \<and>
-      repeat_bod \<xi>' n f g \<sigma>'' \<sigma>' \<tau>a acc' \<tau>o obsv ret)
-  else False)"
+      urepeat_bod \<xi>' n f g \<sigma>'' \<sigma>' \<tau>a acc' \<tau>o obsv ret)))"
+
 
 fun is_uvalfun
   where
@@ -84,8 +75,7 @@ definition repeat
       \<turnstile> (App (uvalfun_to_expr f) (Var 0)) : TPrim Bool) \<and>
     (\<Xi>, [], [option.Some (TRecord [(''acc'', \<tau>a, Present), (''obsv'', \<tau>o, Present)] Unboxed)]
       \<turnstile> (App (uvalfun_to_expr g) (Var 0)) : \<tau>a) \<and>
-    repeat_bod \<xi>' (unat n) (uvalfun_to_expr f) (uvalfun_to_expr g) \<sigma> \<sigma>' \<tau>a acc \<tau>o obsv ret 
-)"
+    urepeat_bod \<xi>' (unat n) (uvalfun_to_expr f) (uvalfun_to_expr g) \<sigma> \<sigma>' \<tau>a acc \<tau>o obsv ret)"
 
 overloading \<xi>1 \<equiv> \<xi>_1
 begin
@@ -94,41 +84,136 @@ definition \<xi>1 :: "(funtyp, abstyp, ptrtyp) uabsfuns"
 "\<xi>1 f x y = (if f = ''repeat_0'' then repeat \<Xi> \<xi>_0 abbreviatedType1 (TPrim (Num U64)) x y  else \<xi>_0 f x y)"
 end
 
-context Generated begin
-
-(*
-lemma valid_ptr_not_in_frame_same:
-  "\<lbrakk>frame \<sigma> w \<sigma>' w'; p \<notin> w; \<sigma> p = option.Some x\<rbrakk> \<Longrightarrow> \<sigma>' p = option.Some x"
-  apply (clarsimp simp: frame_def)
-  apply (erule_tac x = p in allE)
-  apply clarsimp
-  done
-
-lemma readonly_not_in_frame:
-  "\<lbrakk>frame \<sigma> w \<sigma>' w'; \<sigma> p \<noteq> option.None; p \<notin> w\<rbrakk> \<Longrightarrow> p \<notin> w'"
-  "\<lbrakk>frame \<sigma> w \<sigma>' w'; \<forall>p \<in> r. \<sigma> p \<noteq> option.None; r \<inter> w = {}\<rbrakk> \<Longrightarrow> r \<inter> w' = {}"
-   apply (clarsimp simp: frame_def)
-  apply (clarsimp simp: frame_def)
-  apply (rule disjointI)
-  apply (erule_tac x = x in allE; clarsimp)
-  apply (drule_tac x = y in  orthD1; fastforce)
-  done
-
-lemma frame_expand:
-  "\<lbrakk>frame \<sigma> w \<sigma>' w'; \<sigma> p \<noteq> option.None\<rbrakk> \<Longrightarrow> frame \<sigma> (insert p w) \<sigma>' (insert p w')"
-  "\<lbrakk>frame \<sigma> w \<sigma>' w'; \<forall>p\<in>s. \<sigma> p \<noteq> option.None\<rbrakk> \<Longrightarrow> frame \<sigma> (s \<union> w) \<sigma>' (s \<union> w')"
-   apply (clarsimp simp: frame_def)
-   apply (rule conjI; clarsimp)
-  apply (clarsimp simp: frame_def)
-  apply (rule conjI; clarsimp)
-  done
-thm frame_noalias_uval_typing'
-*)
-
-lemma frame_empty:
+lemma (in update_sem) frame_empty:
   "frame \<sigma> {} \<sigma>' {} \<Longrightarrow> \<sigma> = \<sigma>'"
   apply (clarsimp simp: frame_def fun_eq_iff)
   done
+
+context Generated begin
+
+lemma urepeat_bod_preservation:
+  "\<lbrakk>proc_ctx_wellformed \<Xi>';
+    \<xi>' matches-u \<Xi>';
+    \<Xi>', \<sigma> \<turnstile> acc :u \<tau>a \<langle>ra, wa\<rangle>;
+    \<Xi>', \<sigma> \<turnstile> obsv :u \<tau>o \<langle>ro, {}\<rangle>;
+    ro \<inter> wa = {};
+    urepeat_bod \<xi>' n f g \<sigma> \<sigma>' \<tau>a acc \<tau>o obsv ret;
+    \<Xi>', [], [option.Some (TRecord [(''acc'', \<tau>a, Present), (''obsv'', \<tau>o, Present)] Unboxed)] \<turnstile> (App g (Var 0)) : \<tau>a\<rbrakk>
+      \<Longrightarrow> \<exists>r' w'. \<Xi>', \<sigma>' \<turnstile> ret :u \<tau>a \<langle>r', w'\<rangle> \<and> r' \<subseteq> (ra \<union> ro) \<and> frame \<sigma> wa \<sigma>' w'"
+  apply (induct arbitrary: ra wa rule: urepeat_bod.induct[of _ \<xi>' n f g \<sigma> \<sigma>' \<tau>a acc \<tau>o obsv ret])
+   apply (rename_tac \<xi>' f g \<sigma> \<sigma>' \<tau>a acc \<tau>o obsv ret ra wa)
+   apply clarsimp
+   apply (intro exI conjI, assumption, blast, rule frame_id)
+  apply (rename_tac \<xi>' n f g \<sigma> \<sigma>' \<tau>a acc \<tau>o obsv ret ra wa)
+  apply clarsimp
+  apply (case_tac b; clarsimp)
+   apply (intro exI conjI, assumption, blast, rule frame_id)
+  apply (drule_tac x = False in meta_spec; clarsimp)
+  apply (drule_tac x = \<sigma>'' and y = acc' in meta_spec2)
+  apply clarsimp
+  apply (drule_tac \<gamma> = "[URecord [(acc, type_repr \<tau>a), (obsv, type_repr \<tau>o)]]" and
+      \<sigma>' = \<sigma>'' and v = acc' and r = "ra \<union> ro" and w = wa in preservation_mono(1)[rotated -1]; simp?)
+   apply (intro matches_ptrs_some[where r' = "{}" and w' = "{}", simplified]
+      matches_ptrs_empty[where \<tau>s = "[]", simplified])
+   apply (rule u_t_struct; simp?) 
+   apply (intro u_t_r_cons1[where  r' = ro and w' = "{}", simplified]
+      u_t_r_cons1[where  r' = "{}" and w' = "{}", simplified] u_t_r_empty; simp?)
+   apply blast
+  apply clarsimp
+  apply (rename_tac r' w')
+  apply (drule_tac x = r' and y = w' in meta_spec2; simp)
+  apply (erule meta_impE)
+   apply (drule_tac u = obsv in uval_typing_frame(1); simp?)
+  apply (drule meta_mp)
+   apply (drule_tac v = obsv in frame_noalias_uval_typing'(2); simp?)
+  apply clarsimp
+  apply (rename_tac r'' w'')
+  apply (intro exI conjI, assumption)
+   apply blast
+  apply (rule frame_trans; simp?)
+  done
+
+lemma urepeat_bod_early_termination:
+  "\<lbrakk>urepeat_bod \<xi>' i f g \<sigma> \<sigma>' \<tau>a acc \<tau>o obsv ret; i < n;
+    \<xi>', [URecord [(ret, type_repr (bang \<tau>a)), (obsv, type_repr \<tau>o)]]  \<turnstile> (\<sigma>', App f (Var 0)) \<Down>! (\<sigma>', UPrim (LBool True))\<rbrakk>
+    \<Longrightarrow> urepeat_bod \<xi>' n f g \<sigma> \<sigma>' \<tau>a acc \<tau>o obsv ret"
+  apply (induct arbitrary: i rule: urepeat_bod.induct[of _ \<xi>' n f g \<sigma> \<sigma>' \<tau>a acc \<tau>o obsv ret])
+   apply clarsimp
+  apply clarsimp
+  apply (rename_tac i)
+  apply (case_tac i; clarsimp)
+   apply blast
+  apply (case_tac b; clarsimp)
+   apply blast
+  apply (rename_tac ret nat b \<sigma>'' acc')
+  apply (rule_tac x = b in exI)
+  apply (rule conjI; clarsimp)
+  apply (intro exI conjI; assumption)
+  done
+
+declare urepeat_bod.simps[simp del]
+lemma urepeat_bod_step:
+  "\<lbrakk>\<xi>', [URecord [(ret, type_repr (bang \<tau>a)), (obsv, type_repr \<tau>o)]] \<turnstile> (\<sigma>', App f (Var 0)) \<Down>! (\<sigma>', UPrim (LBool False));
+    \<not>(\<xi>', [URecord [(ret, type_repr (bang \<tau>a)), (obsv, type_repr \<tau>o)]] \<turnstile> (\<sigma>', App f (Var 0)) \<Down>! (\<sigma>', UPrim (LBool True)));
+    \<xi>', [URecord [(ret, type_repr \<tau>a), (obsv, type_repr \<tau>o)]] \<turnstile> (\<sigma>', App g (Var 0)) \<Down>! (\<sigma>'', ret');
+    urepeat_bod \<xi>' n f g \<sigma> \<sigma>' \<tau>a acc \<tau>o obsv ret\<rbrakk> 
+    \<Longrightarrow> urepeat_bod \<xi>' (Suc n) f g \<sigma> \<sigma>'' \<tau>a acc \<tau>o obsv ret'"
+  apply (induct arbitrary: \<sigma>'' ret' rule: urepeat_bod.induct[of _ \<xi>' n f g \<sigma> \<sigma>' \<tau>a acc \<tau>o obsv ret])
+   apply (clarsimp simp: urepeat_bod.simps)
+  apply clarsimp
+  apply (erule urepeat_bod.elims; clarsimp)
+  apply (rename_tac \<sigma>'' ret' \<xi> n f g \<sigma> \<sigma>' \<tau>a acc \<tau>o obsv ret b)
+  apply (case_tac b; clarsimp)
+  apply (drule_tac x = b in meta_spec; clarsimp)
+  apply (elim meta_allE meta_impE, assumption, assumption)
+  apply (subst urepeat_bod.simps; clarsimp)
+  apply (rule_tac x = b in exI; clarsimp)
+  apply (intro exI conjI; assumption)
+  done
+declare urepeat_bod.simps[simp]
+
+lemma \<xi>_0_matchesu_\<Xi>:
+  "\<xi>_0 matches-u \<Xi>'"
+  unfolding proc_env_matches_ptrs_def \<xi>0_def
+  by clarsimp
+
+end (* of context *)
+
+lemma (in update_sem) discardable_or_shareable_not_writable:
+assumes "D \<in> k \<or> S \<in> k"
+shows "\<lbrakk> \<Xi>', \<sigma> \<turnstile>  v  :u  \<tau>  \<langle> r , w \<rangle>; K' \<turnstile>  \<tau>  :\<kappa>  k \<rbrakk> \<Longrightarrow> w = {}"
+and   "\<lbrakk> \<Xi>', \<sigma> \<turnstile>* fs :ur \<tau>s \<langle> r , w \<rangle>; K' \<turnstile>* \<tau>s :\<kappa>r k \<rbrakk> \<Longrightarrow> w = {}"
+  using assms
+  by (induct rule: uval_typing_uval_typing_record.inducts)
+    (force simp add: kinding_simps kinding_record_simps kinding_variant_set
+      dest: abs_typing_readonly[where s = Unboxed,simplified])+
+
+lemma (in update_sem) discardable_or_shareable_not_writable':
+shows "\<lbrakk> k = kinding_fn K' \<tau>; D \<in> k \<or> S \<in> k; \<Xi>', \<sigma> \<turnstile>  v  :u  \<tau>  \<langle> r , w \<rangle>; K' \<turnstile>  \<tau>  :\<kappa> k \<rbrakk> \<Longrightarrow> w = {}"
+and   "\<lbrakk> k = (\<Inter>(_,t,b)\<in>set \<tau>s. (case b of Taken \<Rightarrow> UNIV | Present \<Rightarrow> kinding_fn K' t));
+         D \<in> k \<or> S \<in> k; \<Xi>', \<sigma> \<turnstile>* fs :ur \<tau>s \<langle> r , w \<rangle>; K' \<turnstile>* \<tau>s :\<kappa>r k \<rbrakk> \<Longrightarrow> w = {}"
+  by (meson discardable_or_shareable_not_writable)+
+
+(*
+fun repeat_bod
+  where
+"repeat_bod _ 0 _ _ \<sigma> \<sigma>' _ acc _ _ ret = (\<sigma> = \<sigma>' \<and> acc = ret)" |
+"repeat_bod \<xi>' (Suc n) f g \<sigma> \<sigma>' \<tau>a acc \<tau>o obsv ret =
+  (if (\<xi>' , [URecord [(acc, type_repr (bang \<tau>a)), (obsv, type_repr \<tau>o)]] 
+      \<turnstile> (\<sigma>, App f (Var 0)) \<Down>! (\<sigma>, UPrim (LBool True))) \<and>
+      \<not>(\<xi>' , [URecord [(acc, type_repr (bang \<tau>a)), (obsv, type_repr \<tau>o)]] 
+      \<turnstile> (\<sigma>, App f (Var 0)) \<Down>! (\<sigma>, UPrim (LBool False)))
+    then \<sigma> = \<sigma>' \<and> acc = ret
+  else if (\<xi>' , [URecord [(acc, type_repr (bang \<tau>a)), (obsv, type_repr \<tau>o)]] 
+      \<turnstile> (\<sigma>, App f (Var 0)) \<Down>! (\<sigma>, UPrim (LBool False))) \<and>
+      \<not>(\<xi>' , [URecord [(acc, type_repr (bang \<tau>a)), (obsv, type_repr \<tau>o)]] 
+      \<turnstile> (\<sigma>, App f (Var 0)) \<Down>! (\<sigma>, UPrim (LBool True)))
+    then (\<exists>\<sigma>'' acc'. (\<xi>' , [URecord [(acc, type_repr \<tau>a), (obsv, type_repr \<tau>o)]] 
+        \<turnstile> (\<sigma>, App g (Var 0)) \<Down>! (\<sigma>'', acc')) \<and>
+      repeat_bod \<xi>' n f g \<sigma>'' \<sigma>' \<tau>a acc' \<tau>o obsv ret)
+  else False)"
+
+context Generated begin
 
 lemma repeat_bod_preservation:
   "\<lbrakk>proc_ctx_wellformed \<Xi>';
@@ -209,29 +294,7 @@ lemma repeat_bod_step:
   apply (clarsimp simp del: repeat_bod.simps)
   apply (intro exI conjI; assumption)
   done
-
-
-lemma \<xi>_0_matchesu_\<Xi>:
-  "\<xi>_0 matches-u \<Xi>'"
-  unfolding proc_env_matches_ptrs_def \<xi>0_def
-  by clarsimp
-
 end (* of context *)
-
-lemma (in update_sem) discardable_or_shareable_not_writable:
-assumes "D \<in> k \<or> S \<in> k"
-shows "\<lbrakk> \<Xi>', \<sigma> \<turnstile>  v  :u  \<tau>  \<langle> r , w \<rangle>; K' \<turnstile>  \<tau>  :\<kappa>  k \<rbrakk> \<Longrightarrow> w = {}"
-and   "\<lbrakk> \<Xi>', \<sigma> \<turnstile>* fs :ur \<tau>s \<langle> r , w \<rangle>; K' \<turnstile>* \<tau>s :\<kappa>r k \<rbrakk> \<Longrightarrow> w = {}"
-  using assms
-  by (induct rule: uval_typing_uval_typing_record.inducts)
-    (force simp add: kinding_simps kinding_record_simps kinding_variant_set
-      dest: abs_typing_readonly[where s = Unboxed,simplified])+
-
-lemma (in update_sem) discardable_or_shareable_not_writable':
-shows "\<lbrakk> k = kinding_fn K' \<tau>; D \<in> k \<or> S \<in> k; \<Xi>', \<sigma> \<turnstile>  v  :u  \<tau>  \<langle> r , w \<rangle>; K' \<turnstile>  \<tau>  :\<kappa> k \<rbrakk> \<Longrightarrow> w = {}"
-and   "\<lbrakk> k = (\<Inter>(_,t,b)\<in>set \<tau>s. (case b of Taken \<Rightarrow> UNIV | Present \<Rightarrow> kinding_fn K' t));
-         D \<in> k \<or> S \<in> k; \<Xi>', \<sigma> \<turnstile>* fs :ur \<tau>s \<langle> r , w \<rangle>; K' \<turnstile>* \<tau>s :\<kappa>r k \<rbrakk> \<Longrightarrow> w = {}"
-  by (meson discardable_or_shareable_not_writable)+
-
+*)
 
 end
