cogent/examples/repeat/RepeatCorrespondence.thy
@@ -4,6 +4,164 @@ begin
 
 context correspondence_init begin
 
+inductive_cases u_v_primE'     [elim] : "\<Xi>', \<sigma> \<turnstile> UPrim l \<sim> x : TPrim \<tau> \<langle>r, w\<rangle>"
+
+lemma uvrepeat_bod_monocorrespondence:
+  "\<lbrakk>proc_ctx_wellformed \<Xi>';
+    \<xi>u \<sim> \<xi>v matches-u-v \<Xi>';
+    \<Xi>', \<sigma> \<turnstile> uacc \<sim> vacc : \<tau>a \<langle>ra, wa\<rangle>;
+    \<Xi>', \<sigma> \<turnstile> uobsv \<sim> vobsv : \<tau>o \<langle>ro, {}\<rangle>;
+    ro \<inter> wa = {};
+    urepeat_bod \<xi>u n f g \<sigma> \<sigma>' \<tau>a uacc \<tau>o uobsv uret;
+    vrepeat_bod \<xi>v n f g vacc vobsv vret;
+    \<Xi>', [], [option.Some (TRecord [(''acc'', bang \<tau>a, Present), (''obsv'', \<tau>o, Present)] Unboxed)] \<turnstile> (App f (Var 0)) : TPrim Bool;
+    \<Xi>', [], [option.Some (TRecord [(''acc'', \<tau>a, Present), (''obsv'', \<tau>o, Present)] Unboxed)] \<turnstile> (App g (Var 0)) : \<tau>a\<rbrakk>
+      \<Longrightarrow>\<exists>r' w'.  \<Xi>', \<sigma>' \<turnstile> uret \<sim> vret : \<tau>a \<langle>r', w'\<rangle> \<and> r' \<subseteq> (ra \<union> ro) \<and> upd.frame \<sigma> wa \<sigma>' w'"
+  apply (induct n arbitrary: \<sigma> uacc ra wa vacc)
+   apply clarsimp
+   apply (intro exI conjI; simp?)
+    apply blast
+   apply (rule upd.frame_id)
+  apply clarsimp
+  apply (case_tac b; clarsimp)
+   apply (drule_tac r = "(ra \<union> wa) \<union> ro"  and w = "{}" in mono_correspondence(1)[rotated 3]; simp?)
+    apply (intro u_v_matches_some[where r' = "{}" and w' = "{}", simplified]
+                  u_v_matches_empty[where \<tau>s = "[]", simplified]
+                  u_v_struct
+                  u_v_r_cons1[where w' = "{}", simplified]
+                  u_v_r_cons1[where r' = "{}" and w' = "{}", simplified]
+                  u_v_r_empty; simp?)
+    apply (rule upd_val_rel_bang(1); simp)
+   apply clarsimp
+   apply (erule u_v_primE; clarsimp)
+   apply (intro exI conjI; simp?)
+    apply blast
+   apply (rule upd.frame_id)
+  apply (drule_tac r = "(ra \<union> wa) \<union> ro"  and w = "{}" in mono_correspondence(1)[rotated 3]; simp?)
+  apply (intro u_v_matches_some[where r' = "{}" and w' = "{}", simplified]
+                  u_v_matches_empty[where \<tau>s = "[]", simplified]
+                  u_v_struct
+                  u_v_r_cons1[where w' = "{}", simplified]
+                  u_v_r_cons1[where r' = "{}" and w' = "{}", simplified]
+                  u_v_r_empty; simp?)
+   apply (rule upd_val_rel_bang(1); simp)
+  apply clarsimp
+  apply (erule u_v_primE; clarsimp)
+  apply (drule_tac r = "ra \<union> ro"  and w = wa and 
+      \<gamma> = "[URecord [(uacc, type_repr \<tau>a), (uobsv, type_repr \<tau>o)]]" in mono_correspondence(1)[rotated 3]; simp?)
+   apply (intro u_v_matches_some[where r' = "{}" and w' = "{}", simplified]
+                u_v_matches_empty[where \<tau>s = "[]", simplified]
+                u_v_struct
+                u_v_r_cons1[where w' = "{}", simplified]
+                u_v_r_cons1[where r' = "{}" and w' = "{}", simplified]
+                u_v_r_empty; simp?)
+   apply blast
+  apply clarsimp
+  apply (rename_tac r' w')
+  apply (thin_tac "upd.frame _ {} _ {}")
+  apply (frule_tac u = uobsv and v = vobsv in upd_val_rel_frame(1)[rotated 3]; simp?; clarsimp?)
+  apply (frule_tac v = uobsv and v' = vobsv in frame_noalias_upd_val_rel'(2); simp?)
+  apply (elim meta_allE meta_impE, assumption, assumption, assumption, assumption, assumption)
+  apply clarsimp
+  apply (intro exI conjI, assumption, blast)
+  apply (erule upd.frame_trans; assumption)
+  done
+
+lemma uvrepeat_bod_val_executes_from_upd_executes:
+  "\<lbrakk>proc_ctx_wellformed \<Xi>';
+    \<xi>u \<sim> \<xi>v matches-u-v \<Xi>';
+    \<Xi>', \<sigma> \<turnstile> uacc \<sim> vacc : \<tau>a \<langle>ra, wa\<rangle>;
+    \<Xi>', \<sigma> \<turnstile> uobsv \<sim> vobsv : \<tau>o \<langle>ro, {}\<rangle>;
+    ro \<inter> wa = {};
+    urepeat_bod \<xi>u n f g \<sigma> \<sigma>' \<tau>a uacc \<tau>o uobsv uret;
+    \<Xi>', [], [option.Some (TRecord [(''acc'', bang \<tau>a, Present), (''obsv'', \<tau>o, Present)] Unboxed)] \<turnstile> (App f (Var 0)) : TPrim Bool;
+    \<Xi>', [], [option.Some (TRecord [(''acc'', \<tau>a, Present), (''obsv'', \<tau>o, Present)] Unboxed)] \<turnstile> (App g (Var 0)) : \<tau>a\<rbrakk>
+      \<Longrightarrow> \<exists>vret. vrepeat_bod \<xi>v n f g vacc vobsv vret"
+  apply (induct n arbitrary: \<sigma> uacc ra wa vacc)
+   apply clarsimp
+   apply (intro exI; simp)
+  apply clarsimp
+  apply (case_tac b; clarsimp)
+   apply (rule_tac x = vacc in exI)
+   apply clarsimp
+   apply (rule_tac x = b in exI)
+   apply clarsimp
+   apply (frule_tac r = "(ra \<union> wa) \<union> ro"  and w = "{}" and
+      \<gamma>' = "[VRecord [vacc, vobsv]]" in val_executes_from_upd_executes(1)[rotated 3]; simp?)
+    apply (intro u_v_matches_some[where r' = "{}" and w' = "{}", simplified]
+                  u_v_matches_empty[where \<tau>s = "[]", simplified]
+                  u_v_struct
+                  u_v_r_cons1[where w' = "{}", simplified]
+                  u_v_r_cons1[where r' = "{}" and w' = "{}", simplified]
+                  u_v_r_empty; simp?)
+    apply (rule upd_val_rel_bang(1); simp)
+   apply clarsimp
+   apply (frule_tac r = "(ra \<union> wa) \<union> ro"  and w = "{}" in mono_correspondence(1)[rotated 3]; simp?)
+    apply (intro u_v_matches_some[where r' = "{}" and w' = "{}", simplified]
+                  u_v_matches_empty[where \<tau>s = "[]", simplified]
+                  u_v_struct
+                  u_v_r_cons1[where w' = "{}", simplified]
+                  u_v_r_cons1[where r' = "{}" and w' = "{}", simplified]
+                  u_v_r_empty; simp?)
+    apply (rule upd_val_rel_bang(1); simp)
+   apply clarsimp
+   apply (erule u_v_primE'; clarsimp)
+  apply (frule_tac r = "(ra \<union> wa) \<union> ro"  and w = "{}" and
+      \<gamma>' = "[VRecord [vacc, vobsv]]" in val_executes_from_upd_executes(1)[rotated 3]; simp?)
+    apply (intro u_v_matches_some[where r' = "{}" and w' = "{}", simplified]
+                  u_v_matches_empty[where \<tau>s = "[]", simplified]
+                  u_v_struct
+                  u_v_r_cons1[where w' = "{}", simplified]
+                  u_v_r_cons1[where r' = "{}" and w' = "{}", simplified]
+                  u_v_r_empty; simp?)
+   apply (rule upd_val_rel_bang(1); simp)
+  apply clarsimp
+  apply (frule_tac r = "(ra \<union> wa) \<union> ro"  and w = "{}" in mono_correspondence(1)[rotated 3]; simp?)
+   apply (intro u_v_matches_some[where r' = "{}" and w' = "{}", simplified]
+                  u_v_matches_empty[where \<tau>s = "[]", simplified]
+                  u_v_struct
+                  u_v_r_cons1[where w' = "{}", simplified]
+                  u_v_r_cons1[where r' = "{}" and w' = "{}", simplified]
+                  u_v_r_empty; simp?)
+   apply (rule upd_val_rel_bang(1); simp)
+  apply clarsimp
+  apply (erule u_v_primE'; clarsimp)
+  apply (thin_tac "upd.frame _ {} _ {}")
+  apply (frule_tac r = "ra \<union> ro"  and w = wa and
+      \<gamma>' = "[VRecord [vacc, vobsv]]" and
+      e = "App g (Var 0)" in val_executes_from_upd_executes(1)[rotated 3]; simp?)
+   apply (intro u_v_matches_some[where r' = "{}" and w' = "{}", simplified]
+                  u_v_matches_empty[where \<tau>s = "[]", simplified]
+                  u_v_struct
+                  u_v_r_cons1[where w' = "{}", simplified]
+                  u_v_r_cons1[where r' = "{}" and w' = "{}", simplified]
+                  u_v_r_empty; simp?)
+   apply blast
+  apply clarsimp
+  apply (frule_tac r = "ra \<union> ro"  and w = wa and
+      \<gamma>' = "[VRecord [vacc, vobsv]]" and
+      e = "App g (Var 0)" in mono_correspondence(1)[rotated 3]; simp?)
+   apply (intro u_v_matches_some[where r' = "{}" and w' = "{}", simplified]
+                  u_v_matches_empty[where \<tau>s = "[]", simplified]
+                  u_v_struct
+                  u_v_r_cons1[where w' = "{}", simplified]
+                  u_v_r_cons1[where r' = "{}" and w' = "{}", simplified]
+                  u_v_r_empty; simp?)
+   apply blast
+  apply clarsimp
+  apply (frule_tac u = uobsv and v = vobsv in upd_val_rel_frame(1)[rotated 3]; simp?; clarsimp?)
+  apply (drule_tac v = uobsv and v' = vobsv in frame_noalias_upd_val_rel'(2)[rotated 1]; simp?)
+  apply (elim meta_allE meta_impE, assumption, assumption, assumption, assumption)
+  apply clarsimp
+  apply (rename_tac ret)
+  apply (rule_tac x = ret in exI)
+  apply clarsimp
+  apply (rule_tac x = b in exI)
+  apply clarsimp
+  apply (intro exI conjI; assumption)
+  done
+
+(*
 lemma repeat_bod_monocorrespondence:
   "\<lbrakk>proc_ctx_wellformed \<Xi>';
     \<xi>u \<sim> \<xi>v matches-u-v \<Xi>';
@@ -11,7 +169,7 @@ lemma repeat_bod_monocorrespondence:
     \<Xi>', \<sigma> \<turnstile> uobsv \<sim> vobsv : \<tau>o \<langle>ro, {}\<rangle>;
     ro \<inter> wa = {};
     repeat_bod \<xi>u n f g \<sigma> \<sigma>' \<tau>a uacc \<tau>o uobsv uret;
-    vrepeat_bod \<xi>v n f g vacc vobsv vret;
+    repeat_bod' \<xi>v n f g vacc vobsv vret;
     \<Xi>', [], [option.Some (TRecord [(''acc'', bang \<tau>a, Present), (''obsv'', \<tau>o, Present)] Unboxed)] \<turnstile> (App f (Var 0)) : TPrim Bool;
     \<Xi>', [], [option.Some (TRecord [(''acc'', \<tau>a, Present), (''obsv'', \<tau>o, Present)] Unboxed)] \<turnstile> (App g (Var 0)) : \<tau>a\<rbrakk>
       \<Longrightarrow>\<exists>r' w'.  \<Xi>', \<sigma>' \<turnstile> uret \<sim> vret : \<tau>a \<langle>r', w'\<rangle> \<and> r' \<subseteq> (ra \<union> ro) \<and> upd.frame \<sigma> wa \<sigma>' w'"
@@ -66,7 +224,7 @@ lemma repeat_bod_monocorrespondence:
   apply (erule upd.frame_trans; assumption)
   done
 
-inductive_cases u_v_primE'     [elim] : "\<Xi>', \<sigma> \<turnstile> UPrim l \<sim> x : TPrim \<tau> \<langle>r, w\<rangle>"
+
 
 lemma repeat_bod_val_executes_from_upd_executes:
   "\<lbrakk>proc_ctx_wellformed \<Xi>';
@@ -77,7 +235,7 @@ lemma repeat_bod_val_executes_from_upd_executes:
     repeat_bod \<xi>u n f g \<sigma> \<sigma>' \<tau>a uacc \<tau>o uobsv uret;
     \<Xi>', [], [option.Some (TRecord [(''acc'', bang \<tau>a, Present), (''obsv'', \<tau>o, Present)] Unboxed)] \<turnstile> (App f (Var 0)) : TPrim Bool;
     \<Xi>', [], [option.Some (TRecord [(''acc'', \<tau>a, Present), (''obsv'', \<tau>o, Present)] Unboxed)] \<turnstile> (App g (Var 0)) : \<tau>a\<rbrakk>
-      \<Longrightarrow> \<exists>vret. vrepeat_bod \<xi>v n f g vacc vobsv vret"
+      \<Longrightarrow> \<exists>vret. repeat_bod' \<xi>v n f g vacc vobsv vret"
   apply (induct n arbitrary: \<sigma> uacc ra wa vacc)
    apply clarsimp
    apply (rule_tac x = vacc in exI)
@@ -203,13 +361,6 @@ lemma repeat_bod_val_executes_from_upd_executes:
   apply clarsimp
   apply (erule u_v_primE; clarsimp)
   done
-
-lemma
- "\<lbrakk>(\<xi>u, [u] \<turnstile> (\<sigma>, App f (Var 0)) \<Down>! (\<sigma>', UPrim (LBool True))) \<longrightarrow>
-    \<not>(\<xi>u, [u] \<turnstile> (\<sigma>, App f (Var 0)) \<Down>! (\<sigma>', UPrim (LBool False)))\<rbrakk>
-  \<Longrightarrow>
-    (\<xi>v , [v] \<turnstile> App f (Var 0) \<Down> VPrim (LBool True)) \<longrightarrow>
-        \<not> (\<xi>v , [v] \<turnstile> App f (Var 0) \<Down> VPrim (LBool False))"
-  oops
+*)
 end (* of context *)
 end
